dafny/boolean_algebra/evaluation.dfy
@@ -1,29 +1,26 @@
- include "interpretation.dfy"
+ include "expression.dfy"
  
  module evaluation
  {
      import opened expression
-     import opened interpretation
 
     /*
     Evaluate a Boolean expression in a given environment. 
     The recursive structure of this algorithm reflects the
     inductive structure of the expressions we've defined.
     */
-    function method Beval(e: Bexp, i: Binterp): (r: bool) 
+    function method bEval(e: bExp): bool
     {
         match e 
         {
             // Evaluate literal expressions to corresponding values
-            case litExp(b: bool) => b
+            case bTrue => true
+            case bFalse => false
         
-            // Evaluate variable expressions by lookup in environment
-            case varExp(v: Bvar) => lookup(v,i)
-
             // Evaluate operator exprs recursively in same environment
-            case notExp(e1: Bexp) => !Beval(e1,i)
-            case andExp(e1, e2) => Beval(e1,i) && Beval(e2, i)
-            case orExp(e1, e2) =>  Beval(e1, i) || Beval(e2, i)
+            case bNot(e: bExp) => !bEval(e)
+            case bAnd(e1, e2) => bEval(e1) && bEval(e2)
+            case bOr(e1, e2) =>  bEval(e1) || bEval(e2)
         }
     }    
  }
