dafny/dafny-language/advanced.dfy
@@ -1,4 +1,11 @@
-/* Expressions -- advanced topics, for future consideration
+/*
+At present this file contains only a list of Dafny language
+issues not covered in the material presented to date. We will
+introduce many, though not all, of these topics as needed as
+we go along.
+*/
+
+/* EXPRESSIONS
 
 lambda expressions
 object types
@@ -11,7 +18,7 @@ set comprehension
 map comprehension
 */
 
-/* COMMANDS  -- advanced topics, for future consideration
+/* COMMANDS 
 
 yield
 patterns in update/assignment statements
@@ -26,10 +33,14 @@ calc
 skeleton
 */
 
-/* TYPES -- OO to be discussed in future lectures
+/* TYPES -- OO
 
 Objects (class instances), and traits (to be discussed) are of "reference" types, which is to say, values of these types are stored on the heap. Values of other types, including sets and sequences, are of "value types," which is to say values of these types are stored on the stack; and they're thus always treated as "local" variables. They are passed by value, not reference, when passed as arguments to functions and methods. Value types include the basic scalar types (bool, char, nat, int, real), built-in collection types (set, multiset, seq, string, map, imap), tuple, inductive, and co-inductive types (to be discussed). Reference type values are allocated dynamically on the heap, are passed  by reference, and therefore can be "side effected" (mofified) by methods to which they are passed. They include arrays and objects.
 */
-    
 
+/* OTHER
+
+predicate
+lemma
+*/
  
