dafny/propositional-logic/evaluation.dfy
@@ -1,0 +1,27 @@
+ include "interpretation.dfy"
+ 
+ module evaluation
+ {
+     import opened expression
+     import opened interpretation
+
+    /*
+    Evaluate a propositional expression given an interpretation.
+    The recursive structure of this algorithm again reflects the
+    inductive structure of the expressions defined by the syntax
+    of our language.
+    */
+    function method pEval(e: pExp, i: pInterp): (r: bool) 
+    {
+        match e 
+        {
+            // Evaluate variable expressions by lookup in environment
+            case pVarExp(v: pVar) => lookup(v,i)
+
+            // Evaluate operator exprs recursively in same environment
+            case pNot(e1: pExp) => !pEval(e1,i)
+            case pAnd(e1, e2) => pEval(e1,i) && pEval(e2, i)
+            case pOr(e1, e2) =>  pEval(e1, i) || pEval(e2, i)
+        }
+    }    
+ }
