dafny/propositional-logic/expression.dfy
@@ -1,0 +1,149 @@
+module expression
+{
+    /*
+        Now we define the *syntax* of a little language 
+        of Propositional Logic.
+    */
+
+
+    /*
+    We define an infinite set of "propositional
+    variables" as terms of the form mkVar(s), and 
+    of type, pVar.
+    */
+
+    datatype pVar = mkVar(name: string) 
+
+    /*
+    Note to instructor-self: This method not used.
+    */
+    function method pVar_name(b: pVar): string 
+    {
+        match b
+        {
+            case mkVar(s: string) => s
+        }
+    }
+
+    
+   /*
+   The syntax of our language of propositions.
+   */
+    datatype pExp = 
+        // variable expressions
+        pVarExp (v: pVar) | 
+
+        // operator application expression
+        pNot (e: pExp) |
+        pAnd (e1: pExp, e2: pExp) |
+        pOr (e1: pExp, e2: pExp)
+
+
+    
+    /*
+    The rest of this module implements two methods,
+    one of which returns the *set* of variables in a
+    given expression, and the other of which converts
+    that set into a sequence and returns it. It is 
+    much easier to work with sets than with sequences
+    when collecting the variables in an expression.
+    We don't want to include a variable more than once
+    when the same variable occurs in two sub-expressions.
+    But some of the code that uses this module will need 
+    an ordered collection, i.e., a sequence, of all the
+    variables, so we provide a function that converts a
+    set into a sequence.
+    */
+
+    /*
+    First, given a pExp, return a *set() containing all 
+    and only the variables that appear in the expression. 
+    A set contains a given element at most one time, so 
+    even if a variable appears multiple times in a given
+    expression, it'll be in the resulting set only once.
+    */
+    function method setVarsIn(e: pExp): set<pVar>
+    {
+      /*
+      Do the work by calling a helper function with an
+      empty sequence as the starting value. This "design 
+      pattern" is typical: one implements a call to a
+      a non-recursive function (this one) that then calls 
+      a recursive function with some extra arguments to
+      actually do the work.
+      */
+      setVarsInHelper(e, {})
+    }
+
+    /*
+    This recursive function adds the set of variables in a 
+    given expression to the set, r, given as an argument. So, 
+    to get a set of the variables in a given expression, call 
+    this function with the expression and with an empty set. 
+    This is just what the "top-level" function above does.
+
+    This code exhibits a second fundamental algorithm design
+    pattern: mutual recursion. It doesn't call itself recursively,
+    but, in cases where there's more work to do, calls the top-level 
+    method (that called it). This recursive call to the top level
+    computes the set of variables for the *subexpression* being
+    processed by calling this method again. This method then 
+    combines that result, passed in as *r*, with the results 
+    obtained so far (represented in r) to compute the final 
+    answer. 
+    */
+    function method setVarsInHelper(e: pExp, r: set<pVar>): set<pVar>
+    {
+        match e
+        {
+            // a var expression adds the variable it not yet there
+            case pVarExp (v: pVar) => r + { v }
+  
+            // add, or , and not expression adds the variables below 
+            case pNot (e: pExp) => r + setVarsIn(e)
+            case pAnd (e1: pExp, e2: pExp) =>
+                r + setVarsIn(e1) + setVarsIn(e2)
+            case pOr (e1: pExp, e2: pExp) =>
+                r + setVarsIn(e1) + setVarsIn(e2)
+        }
+    }
+
+    /*
+    This method gets the *set* of variables in a given
+    expression and returns it as an ordered sequence. The
+    order in which the elements will appear is undefined.
+    That is, they will be in some order, but one must not
+    count on there being any particular order. 
+    */
+    method seqVarsIn(e: pExp) returns (result: seq<pVar>)
+    {
+        /* Compute the set of variables the convert to sequence
+           Dafny does not allow expressions in return statements
+           so we compute and store the results of the expression
+           first, and then return
+        */
+
+        result := setVarsToSeq(setVarsIn(e));
+        return /* result */;
+    }
+
+    /*
+    Given a set of propositional variables, convert it into a 
+    sequence in some arbitrary order by calling a recursive 
+    helper function with an initially empty sequence. This is 
+    a second example of the design pattern seen above.
+    */
+    method setVarsToSeq(s: set<pVar>) returns (result: seq<pVar>)
+    {
+        var l: seq<pVar> := [];
+        var s' := s;
+        while (s' != {}) 
+            decreases s';
+        {
+            var v :| v in s';
+            l := [ v ] + l;
+            s' := s' - { v };
+        }
+        return l;
+    }
+}
