dafny/propositional-logic/test_evaluation.dfy
@@ -1,0 +1,48 @@
+include "evaluation.dfy"
+
+
+module bexptest
+{
+    import opened expression
+    import opened interpretation
+    import opened evaluation
+
+    method Main()
+    {
+        /*
+            let's build the expression (P \/ Q) /\ ~R
+            in plain text, that's (P or Q) and (not R)
+        */
+        var P := mkVar("P");
+        var Q := mkVar("Q");
+        var R := mkVar("R");
+    
+        var Pexp := pVarExp(P);
+        var Qexp := pVarExp(Q);
+        var Rexp := pVarExp(R);
+        var notRexp := pNot(Rexp);
+        var PorQexp := pOr(Pexp,Qexp);
+        var PorQandnotRexp := pAnd(PorQexp,notRexp);
+
+        /*
+            Now let's build an "interpretation."
+            This is a binding of variables in our
+            little language to Boolean values, in
+            the form of a map.
+        */
+        var st: pInterp := map[
+                                P := true, 
+                                Q := false, 
+                                R := false
+                               ];
+
+        // Finally, let's do a "smoke test"
+        print "\nThe state is ", st, "\n";
+        print "P is ", pEval(Pexp, st), "\n";
+        print "Q is ", pEval(Qexp, st), "\n";
+        print "R is ", pEval(Rexp, st), "\n";
+        print "notR is ", pEval(notRexp, st), "\n";
+        print "PorQ is ", pEval(PorQexp, st), "\n";
+        print "PorQ_and_notR is ", pEval(PorQandnotRexp, st), "\n\n";
+    }
+}
