dafny/specification/imperative-test.dfy
@@ -11,6 +11,6 @@ method Main()
     print "The (right) factorial of 5 is ", vfac5', "\n";
     var fibu5000' := fibonacci_unverified(5000);
     print "The (wrong) Fibonacci[5000] is ", fibu5000', "\n";
-    var fibv1_000_000' := fibonacci_verified(1_000_000);
-    print "The (right!) Fibonacci[1_000_000] is ", fibv1_000_000', "\n";
+    var fibv100_000' := fibonacci_verified(100_000);
+    print "The (right!) Fibonacci[100_000] is ", fibv100_000', "\n";
 }
