dafny/specification/private.dfy
@@ -1,0 +1,48 @@
+include "functional.dfy"
+
+module homework4
+{
+import opened functional
+method sumto_verified(n: nat) returns (f: nat)
+    ensures f == sumto(n)
+    {
+        var a: nat := 0;
+        var i: nat := n;
+        assert a + sumto(i) == sumto(n);
+        while (i > 0) 
+            invariant a + sumto(i) == sumto(n)
+            decreases i;
+        {
+            a := a + i;
+            i := i - 1;
+        }
+        return a;
+    }
+
+    method sum_squares_verified(n: nat) returns (f: nat)
+        ensures f == sum_squares(n)
+        {
+            var a: nat := 0;
+            var i: nat := n;
+            assert a + sum_squares(i) == sum_squares(n);
+            while (i > 0)
+                invariant 0 <= i <= n;
+                invariant a + sum_squares(i) == sum_squares(n);
+                decreases i;
+            {
+                a := a + (i * i);
+                i := i - 1;
+            }
+            return a;
+        }
+
+    method Main()
+    {
+        print "\n";
+        var n: nat := 5;
+        var r := sumto_verified(n);
+        print "sumto ", n, " is ", r, "\n";
+        r := sum_squares_verified(n);
+        print "sum_squares ", n, " is ", r, "\n";
+    }
+}
