notes/_build/html/_sources/06-boolean-algebra.rst.txt
@@ -1,0 +1,23 @@
+Now we define the *syntax* of a little language 
+of Boolean expressions.
+
+We use the definition of the syntax of Boolean expressions to
+introduce the fundamental concept of inductive definitions.  Inductive
+definitions of data types representing often infinite sets of values
+is done by first defining a set starting values (like base cases for a
+recursion) and then by defining rules for forming new values from ones
+already defined.
+    
+Here the base values are the terms litTrue and litFalse. We will
+eventually interpret them as "literal" terms representing the Boolean
+values, true and false.
+
+
+.. code-block:: dafny
+
+    datatype Bexp = 
+        litTrue |
+        litFalse | 
+        bNotExp (e: Bexp) |
+        bAndExp (e1: Bexp, e2: Bexp) |
+        bOrExp (e1: Bexp, e2: Bexp)
