notes/_build/html/_sources/08-propositional-logic.rst.txt
@@ -1,0 +1,314 @@
+**********************
+8. Propositional Logic
+**********************
+
+A mathematical logic is defined by (1) a *syntax* that specifies the
+set (usually infinite) of *well formed expressions* in the language
+(also called *well formed formulae*, or *wffs*), and (2) a *semantics*
+by which one can evaluate *truth value* of any such expression.
+
+Each sentence in a logical language is intended to represent a *truth
+claim*: an assertion, about the prevailing *state of affairs* in some
+*domain of discourse* that is either true or false. Dafny *assertions*
+are logical expressions in this sense: they assert that the state of a
+program at a specific point in its execution has certain properties
+(e.g., that the value of a loop index is greater than zero) , or that
+a specific relationship always holds between the state of the program
+before and after some code is run (e.g., pre- and post-conditions and
+loop invariants).
+
+To use a logic for practical purposes, one must (1) understand how to
+represent states of affairs in the domain of discourse of interest as
+expressions in the logical language of the logic, and (2) hae some
+means of evaluating the truth values of the resulting expressions. In
+Dafny, one must understand the logical language in which assertions
+and related constructs (such as pre- and post-conditions) are written.
+
+In many cases--the magic of an automated verifier such as Dafny--a
+programmer can rely on Dafny to evaluate truth values of assertions
+automatically. When Dafny is unable to verify the truth of a claim,
+however, the programmer will also have to understand something about
+the way that truth is ascertained in the logic, so as to be able to
+provide Dafny with the help it might need to be able to complete its
+verification task.
+
+In this chapter, we take a major step toward understanding logic and
+proofs by introducing the language *propositional logic* and a means
+of evaluating the truth of any sentence in the language. The language
+is closely related to the language of Boolean expressions introduced
+in the last chapter. The main syntactic difference is that we add a
+notion of *propositional variables*. We will defined the semantics of
+this language by introducing the concept of an *interpration*, which
+specifies a Boolean truth value for each such variable. We will then
+evaluate the truth value of an expression *given an interpration for
+the proposition variables in that expression* by replacing each of the
+variables with its corresponding Boolean value and then using our
+Boolean expression evaluator to determing the truth value of the
+expression.
+
+We will also note that this formulation gives rise to an important new
+set of logical problems. Given an expression, does there exist an
+interpretation that makes that expression evaluate to true? Do all
+interpretations make it value to true? Can it be there there are no
+interpretations that make a given expression evaluate to true?  And,
+finally, are there *efficient* algorithms for *deciding* whether or
+not the answer to any such question is yes or no.
+
+
+Introduction
+============
+
+The rest of this chapter illustrates and further develops these ideas
+using Boolean algebra, and a language of Boolean expressions, as a
+case study in precise definition of the syntax (expression structure)
+and semantics (expression evaluation) of a simple formal language: of
+Boolean expressions containing Boolean variables.
+
+To illustrate the potential utility of this language and its semantics
+we will define three related *decision problems*. A decision problem
+is a *kind* of problem for which there is an algorithm that can solve
+any instance of the problem. The three decision problems we will study
+start with a Boolean expression, one that can contain variables, and
+ask where there is an assignment of *true* and *false* values to the
+variables in the expression to make the overall expression evaluate to
+*true*.
+
+Here's an example. Suppose you're given the Boolean expression,
+:math:`(P \lor Q) \land (\lnot R)`. The top-level operator is
+*and*. The whole expression thus evaluates to *true* if and only if
+both subexpressions do: :math:`(P \lor Q)` and :math:`\land (\lnot
+R)`, respectively. The first, :math:`(P \lor Q)`, evaluates to *true*
+if either of the variables, *P* and *Q*, are set to true. The second
+evaluates to true if and only if the variable *R* is false. There are
+thus settings of the variables that make the formula true. In each of
+them, *R* is *false*, and either or both of *P* and *Q* are set to
+true.
+
+Given a Boolean expression with variables, an *interpretation* for
+that expression is a binding of the variables in that expression to
+corresponding Boolean values. A Boolean expression with no variables
+is like a proposition: it is true or false on its own. An expression
+with one or more variables will be true or false depending on how the
+variables are used in the expression.
+
+An interpretation that makes such a formula true is called a *model*.
+The problem of finding a model is called, naturally enough, the model
+finding problem, and the problem of finding *all* models that make a
+Boolean expression true, the *model enumeration* or *model counting*
+problem.
+
+The first major *decision problem* that we identify is, for any given
+Boolean expression, to determine whether it is *satisfiable*. That is,
+is there at least one interpretation (assignment of truth values to
+the variables in the expression that makes the expression evaluate to
+*true*?  We saw, for example, that the expression, :math:`(P \lor Q)
+\land (\lnot R)` is satifiable, and, moreover, that :math:`\{ (P,
+true), (Q, false), (R, false) \}` is a (one of three) interpretations
+that makes the expression true.
+
+Such an interpretation is called a *model*. The problem of finding a
+model (if there is one), and thereby showing that an expression is
+satisfiable, is naturally enough called the* model finding* problem.
+
+A second problem is to determine whether a Boolean expression is
+*valid*. An expression is valid if *every* interpretation makes the
+expression true. For example, the Boolean expression :math:`P \lor
+\neg P` is always true. If *P* is set to true, the formula becomes
+:math:`true \lor false`. If *P* is set to false, the formula is then
+:math:`true \lor false`. Those are the only two interpretations and
+under either of them, the resulting expression evaluates to true.
+
+A third related problem is to determine whether a Boolean expression
+is it *unsatisfiable*? This case occurs when there is *no* combination
+of variable values makes the expression true. The expression :math:`P
+\land \neg P` is unsatisfiable, for example. There is no value of $P$
+(either *true* or *false*) that makes the resulting formula true.
+
+These decision problems are all solvable. There are algorithms that in
+a finite number of steps can determine answers to all of them. In the
+worst case, one need only look at all possible combinations of true
+and false values for each of the (finite number of) variables in an
+expression. If there are *n* variables, that is at most :math:`2^n`
+combinations of such values. Checking the value of an expression for
+each of these interpretations will determine whether it's satisfiable,
+unsatisfiable, or valid. In this chapter, we will see how these ideas
+can be translated into runnable code.
+
+The much more interesting question is whether there is a fundamentally
+more efficient approach than checking all possible interpretations: an
+approach with a cost that increases *exponentially* in the number of
+variables in an expression. This is the greatest open question in all
+of computer science, and one of the greatest open questions in all of
+mathematics.
+
+So let's see how it all works. The rest of this chapter first defines
+a *syntax* for Boolean expressions. Then it defines a *semantics* in
+the form of a procedure for *evaluating* any given Boolean expression
+given a corresponding *interpretation*, i.e., a mapping from variables
+in the expression to corresponding Boolean values. Next we define a
+procedure that, for any given set of Boolean variables, computes and
+returns a list of *all* interpretations. We also define a procedure
+that, given any Boolean expression returns the set of variables in the
+expression. For ths set we calculate the set of all interpretations.
+Finally, by evaluating the expression on each such interpretation, we
+decide whether the expression is satisfiable, unsatisfiable, or valid.
+
+Along the way, we will meet *inductive definitions* as a fundamental
+approach to concisely specifying languages with a potentially infinite
+number of expressions, and the *match* expression for dealing with
+values of inductively defined types. We will also see uses of several
+of Dafny's built-in abstract data types, including sets, sequences,
+and maps. So let's get going.
+
+
+Syntax
+=====
+
+Any basic introduction to programming will have made it clear that
+there is an infinite set of Boolean expressions. First, we can take
+the Boolean values, *true* and *false*, as *literal* expressions.
+Second, we can take *Boolean variables*, such as *P* or *Q*, as a
+Boolean *variable* expressions. Finally, we take take each Boolean
+operator as having an associated expression constructor that takes one
+or more smaller *Boolean expressions* as arguments.
+
+Notice that in this last step, we introduced the idea of constructing
+larger Boolean expressions out of smaller ones. We are thus defining
+the set of all Boolean expressions *inductively*. For example, if *P*
+is a Boolean variable expression, then we can construct a valid larger
+expression, :math:`P \land true` to express the conjunction of the
+value of *P* (whatever it might be( with the value, *true*. From here
+we could build the larger expression, *P \lor (P \land true)*, and so
+on, ad infinitum.
+
+We define an infinite set of "variables" as terms of the form
+mkVar(s), where s, astring, represents the name of the variable. The
+term mkVar("P"), for example, is our way of writing "the var named P."
+
+.. code-block:: dafny
+
+    datatype Bvar = mkVar(name: string) 
+
+
+Here's the definition of the *syntax*:
+
+.. code-block:: dafny
+
+    datatype Bexp = 
+        litExp (b: bool) | 
+        varExp (v: Bvar) | 
+        notExp (e: Bexp) |
+        andExp (e1: Bexp, e2: Bexp) |
+        orExp (e1: Bexp, e2: Bexp)
+
+Boolean expresions, as we've defined them here, are like propositions
+with paramaters. The parameters are the variables. Depending on how we
+assign them *true* and *false* values, the overall proposition might be
+rendered true or false.
+
+Semantics
+=========
+
+Interpretations
+---------------
+
+
+Evaluate a Boolean expression in a given environment.  The recursive
+structure of this algorithm reflects the inductive structure of the
+expressions we've defined.
+
+.. code-block:: dafny
+
+    type interp = map<Bvar, bool>
+
+
+Evaluation
+----------
+
+.. code-block:: dafny
+
+    function method Beval(e: Bexp, i: interp): (r: bool) 
+    {
+        match e 
+        {
+            case litExp(b: bool) => b
+            case varExp(v: Bvar) => lookup(v,i)
+            case notExp(e1: Bexp) => !Beval(e1,i)
+            case andExp(e1, e2) => Beval(e1,i) && Beval(e2, i)
+            case orExp(e1, e2) =>  Beval(e1, i) || Beval(e2, i)
+        }
+    }    
+}
+
+
+Lookup value of given variable, v, in a given interpretation, i. If
+there is not value for v in i, then just return false. This is not a
+great design, in that a return of false could mean one of two things,
+and it's ambiguous: either the value of the variable really is false,
+or it's undefined.  For now, though, it's good enough to illustate our
+main points.
+
+.. code-block:: dafny
+
+    function method lookup(v: Bvar, i: interp): bool
+    {
+        if (v in i) then i[v]
+        else false
+    }
+
+Now that we know the basic values and operations of Boolean algebra,
+we can be precise about the forms of and valid ways of transforming
+*Boolean expressions.* For example, we've seen that we can transform
+the expression *true and true* into *true*. But what about *true and
+((false xor true) or (not (false implies true)))*?
+
+To make sense of such expressions, we need to define what it means for
+one to be well formed, and how to evaluate any such well formed
+expressions by transforming it repeatedly into simpler forms but in
+ways that preserve its meaning until we reach a single Boolean value.
+
+Decision Problems
+=================
+
+It is now possible for you to understand what is the most important
+*open question* (unsolved mathematical problem) in computer science.
+Is there an *efficient* algorithm for determining whether any given
+Boolean formula is satisfiable?
+
+whether there is a combination of Boolean
+variable values that makes any given Boolean expression true is the
+most important unsolved problem in computer science. We currently do
+not know of a solution that with runtime complexity that is better
+than exponential the number of variables in an expression.  It's easy
+to determine whether an assignment of values to variables does the
+trick: just evaluate the expression with those values for the
+variables. But *finding* such a combination today requires, for the
+hardest of these problems, trying all :math:``2^n`` combinations of
+Boolean values for *n* variables.
+
+At the same time, we do not know that there is *not* a more efficient
+algorithm. Many experts would bet that there isn't one, but until we
+know for sure, there is a tantalizing possibility that someone someday
+will find an *efficient decision procedure* for Boolean satisfiability.
+
+To close this exploration of computational complexity theory, we'll
+just note that we solved an instances of another related problem: not
+only to determine whether there is at least one (whether *there
+exists*) at least one combination of variable values that makes the
+expression true, but further determining how many different ways there
+are to do it.
+
+Researchers and advanced practitioners of logic and computation
+sometimes use the word *model* to refer to a combination of variable
+values that makes an expression true. The problem of finding a Boolean
+expression that *satisfies* a Boolean formula is thus somtetimes
+called the *model finding* problem. By contrast, the problem of
+determining how many ways there are to satisfy a Boolean expression is
+called the *model counting* problem.
+
+Solutions to these problems have a vast array of practical uses.  As
+one still example, many logic puzzles can be represented as Boolean
+expressions, and a model finder can be used to determine whether there
+are any "solutions", if so, what one solution is. 
+
+
